src/QUIC.Impl.PacketNumber.fsti
@@ -1,6 +1,7 @@
 module QUIC.Impl.PacketNumber
 include QUIC.Spec.PacketNumber
 open QUIC.Spec.Base
+open QUIC.Impl.Base
 open LowParse.Low.Writers
 
 module U64 = FStar.UInt64
@@ -8,18 +9,19 @@ module U32 = FStar.UInt32
 module HST = FStar.HyperStack.ST
 module B = LowStar.Buffer
 module HS = FStar.HyperStack
+module SecretIntegers = Lib.IntTypes
 
 inline_for_extraction
 val validate_packet_number
   (last: last_packet_number_t)
   (pn_len: packet_number_length_t)
-: Tot (validator (parse_packet_number last pn_len))
+: Tot (validator (parse_packet_number last (u32_of_pnl pn_len)))
 
 inline_for_extraction
 val jump_packet_number
   (last: last_packet_number_t)
   (pn_len: packet_number_length_t)
-: Tot (jumper (parse_packet_number last pn_len))
+: Tot (jumper (parse_packet_number last (u32_of_pnl pn_len)))
 
 inline_for_extraction
 val read_packet_number
@@ -29,14 +31,14 @@ val read_packet_number
   (#rel: _)
   (sl: slice rrel rel)
   (pos: U32.t)
-: HST.Stack (packet_number_t last pn_len)
+: HST.Stack (packet_number_t last (u32_of_pnl pn_len))
   (requires (fun h ->
     live_slice h sl /\
     U32.v pos + 4 <= U32.v sl.len
   ))
   (ensures (fun h res h' ->
     B.modifies B.loc_none h h' /\
-    valid_content (parse_packet_number last pn_len) h sl pos res
+    valid_content (parse_packet_number last (u32_of_pnl pn_len)) h sl pos res
   ))
 
 inline_for_extraction
@@ -44,8 +46,8 @@ noextract
 val swrite_packet_number
   (last: last_packet_number_t)
   (pn_len: packet_number_length_t)
-  (pn: packet_number_t last pn_len)
+  (pn: packet_number_t last (u32_of_pnl pn_len))
   (h0: HS.mem)
   (sout: slice (srel_of_buffer_srel (B.trivial_preorder _)) (srel_of_buffer_srel (B.trivial_preorder _)))
   (pout_from0: U32.t)
-: Tot (y: swriter (serialize_packet_number last pn_len) h0 (4 - U32.v pn_len) sout pout_from0 { swvalue y == pn })
+: Tot (y: swriter (serialize_packet_number last (u32_of_pnl pn_len)) h0 (4 - SecretIntegers.v pn_len) sout pout_from0 { swvalue y == pn })
